@prefix owl: <http://www.w3.org/2002/07/owl#> .
@prefix rdfs: <http://www.w3.org/2000/01/rdf-schema#> .
@prefix xsd: <http://www.w3.org/2001/XMLSchema#> .
@prefix ids: <https://w3id.org/idsa/core/> .
@prefix idsm: <https://w3id.org/idsa/metamodel/> .

# Classes
# -------

ids:DataApp
    a owl:Class; 
    idsm:abstract true;
    rdfs:label "DataApp"@en;
    rdfs:comment "Self-contained, self-descriptive software package that is distributed via the App Store and deployed inside a Connector; provides access to data and data processing capaÂ­bilities; the interface of a Data App is semantically described by the IDS Information Model."@en;.
    # Purpose: mediation and processing of "data"
    # rdfs:comment "Data processing or mediating software executed within the Connector runtime."@en .
    # TODO: exposes at least one interface

ids:SystemAdapter
    a owl:Class;
    rdfs:subClassOf ids:DataApp;
    rdfs:label "System Adapter"@en;
    rdfs:comment "Data Apps that integrate sources and sinks of digital content maintained internally on Participant's premises with a Connector."@en.
    # May offer Data Processing capabilities, therefore not defined as disjoint

ids:DataProcessingApp
    a owl:Class;
    rdfs:subClassOf ids:DataApp;
    rdfs:label "DataProcessingApp"@en;
    rdfs:comment "Data App for a (stateless) processing of digital content according to exposed software interfaces."@en.

ids:DataAppPlugin
    a owl:Class;
    rdfs:subClassOf ids:Software;
    rdfs:label "DataApp Plugin"@en;
    rdfs:comment "Add-on software extending a host Data App with a dedicated capability. The plugin depends on a particular version (range) of the host Data App which governs its integration, configuration and life-cycle."@en.

ids:DataAppAsset
    a owl:Class;
    rdfs:subClassOf ids:Software;
    rdfs:label "DataApp Asset"@en;
    rdfs:comment "Script code, algorithm or any other kind of interpreted software."@en.


ids:appDescription
    a owl:ObjectProperty ;
    rdfs:label "app description" @en ;
    rdfs:comment "References the corresponding ids:Resource, which contains descriptive metadata about the app." @en ;
    rdfs:domain ids:DataApp ;
    rdfs:range ids:SoftwareResource ;
.

ids:appEndpoint
    a owl:ObjectProperty ;
    rdfs:label "app endpoint" @en;
    rdfs:comment "References endpoints of a App. Based on the app type, input, config, output endpoints need to be defined. See ids:AppEndpoint for details on endpoint description." @en;
    rdfs:domain ids:DataApp ;
    rdfs:range ids:AppEndpoint ;
    .
    