@prefix owl: <http://www.w3.org/2002/07/owl#> .
@prefix rdfs: <http://www.w3.org/2000/01/rdf-schema#> .
@prefix xsd: <http://www.w3.org/2001/XMLSchema#> .
@prefix ids: <https://w3id.org/idsa/core/> .
@prefix idsm: <https://w3id.org/idsa/metamodel/> .
@prefix skos: <http://www.w3.org/2004/02/skos/core#> .

# Classes
# -------

ids:DataApp
    a owl:Class; 
    idsm:abstract true;
    rdfs:label "DataApp"@en;
    rdfs:comment """Self-contained, self-descriptive software package that is distributed via the App Store and deployed
        inside a Connector; provides access to data and data processing capabilities; the interface of a Data App is
        semantically described by the IDS Information Model."""@en;.


ids:SystemAdapterApp
    a owl:Class;
    rdfs:subClassOf ids:DataApp;
    rdfs:label "System Adapter App"@en;
    rdfs:comment "Data Apps that integrate sources and/or sinks of digital content maintained internally on Participant's premises with a Connector."@en.

ids:SmartDataApp 
    a owl:Class;
    rdfs:subClassOf ids:DataApp;
    rdfs:label "Smart Data App"@en;
    rdfs:comment "Smart Data App for processing of digital content according to exposed software interfaces."@en.

ids:OrchestrationApp 
    a owl:Class;
    rdfs:subClassOf ids:DataApp;
    rdfs:label "Orchestration App"@en;
    rdfs:comment "App for orchestration Apps in an ids:Connector."@en.


#ids:DataAppPlugin
#    a owl:Class;
#    rdfs:subClassOf ids:Software;
#    rdfs:label "DataApp Plugin"@en;
#    rdfs:comment "Add-on software extending a host Data App with a dedicated capability. The plugin depends on a particular version (range) of the host Data App which governs its integration, configuration and life-cycle."@en.

#ids:DataAppAsset
#    a owl:Class;
#    rdfs:subClassOf ids:Software;
#    rdfs:label "DataApp Asset"@en;
#    rdfs:comment "Script code, algorithm or any other kind of interpreted software."@en.


ids:appDescription
    a owl:ObjectProperty ;
    rdfs:label "app description" @en ;
    rdfs:comment "References the corresponding ids:Resource, which contains descriptive metadata about the app." @en ;
    rdfs:domain ids:DataApp ;
    rdfs:range ids:AppResource ;
.

ids:appEndpoint
    a owl:ObjectProperty ;
    rdfs:label "app endpoint" @en;
    rdfs:comment "References endpoints of a App. Based on the app type, input, config, output endpoints need to be defined. See ids:AppEndpoint for details on endpoint description." @en;
    rdfs:domain ids:DataApp ;
    rdfs:range ids:AppEndpoint ;
    .
    
ids:appDocumentation
    a owl:DatatypeProperty ;
    rdfs:label "app Api documentation"@en ;
    rdfs:comment """IRI reference to App documentation. An App may have multiple documentations, e.g.,
    an overall usage documentation, as well as endpoint-specific API documentations.""" @en;
    rdfs:domain [owl:unionOf 
        (ids:DataApp ids:AppEndpoint ids:AppResource)
        ] ;
    rdfs:range xsd:anyURI ;
.