@prefix rdf:   <http://www.w3.org/1999/02/22-rdf-syntax-ns#> .
@prefix owl: <http://www.w3.org/2002/07/owl#> .
@prefix rdfs: <http://www.w3.org/2000/01/rdf-schema#> .
@prefix xsd: <http://www.w3.org/2001/XMLSchema#> .
@prefix dcat: <http://www.w3.org/ns/dcat#> .
@prefix ids: <https://w3id.org/idsa/core/> .
@prefix idsc: <https://w3id.org/idsa/code/> .
@prefix idsm: <https://w3id.org/idsa/metamodel/> .

# Classes
# -------

ids:ConfigurationModel
    a owl:Class;
    # As a subclass of ids:Described, ConfigurationModel gains title and description properties
    rdfs:subClassOf ids:Described ;     
    rdfs:label "Configuration Model." @en ;
    rdfs:comment "A Model to represent a Connector's configuration." @en ;
    .

ids:ConnectorDeployMode
    a owl:Class;
    rdfs:label "Connector Deploy Mode" @en;
    rdfs:comment "Instances of this class describe the connector's deployement mode, e.g, if a Connector is deployed " @en;
    .

ids:ConnectorStatus
    a owl:Class;
    rdfs:label "Connector Status" @en;
    rdfs:comment "Instances of this class describe the connector's current status. Statuses may include ONLINE, OFFLINE or BAD_CONFIGURED. " @en;
    .
    
ids:LogLevel
    a owl:Class;
    rdfs:label "Log Level" @en;
    rdfs:comment "Instances of this class describe the log level of the Configuration Model. Log levels may include NONE, MINIMAL or DEBUG. " @en;
    .
    
# Properties
# ----------

ids:connectorDeployMode
    a owl:ObjectProperty;
    rdfs:label "connector Deploy Mode"@en;
    rdfs:domain ids:ConfigurationModel;
    rdfs:range ids:ConnectorDeployMode;
    rdfs:comment "Deploy mode of a Connector, e.g., test deployment vs. productive deployment."@en.

# TODO: necessary? 
ids:connectorStatus
    a owl:ObjectProperty;
    rdfs:label "connector Status"@en;
    rdfs:domain ids:ConfigurationModel;
    rdfs:range ids:ConnectorStatus;
    rdfs:comment "Status of the connector."@en.

ids:connectorProxy
    a owl:DatatypeProperty;
    rdfs:domain ids:ConfigurationModel;
    rdfs:range ids:Proxy;
    rdfs:label "connector proxy"@en ;
    rdfs:comment "The proxy an ids:Connector uses for network communication."@en ;
    .

ids:logLevel
    a owl:ObjectProperty;
    rdfs:domain ids:ConfigurationModel;
    rdfs:range ids:LogLevel;
    rdfs:label "log level";
    rdfs:comment "Configuration Model log Level. ";
    .
    
ids:trustStore
    a owl:DatatypeProperty;
    rdfs:label "trust Store";
    rdfs:comment "Path to Trust Store containing necessary Connector certificates";
    rdfs:domain ids:ConfigurationModel;
    rdfs:range xsd:anyURI;
    .

ids:keyStore
    a owl:DatatypeProperty;
    rdfs:label "key Store";
    rdfs:domain ids:ConfigurationModel ;
    rdfs:range xsd:anyURI;
    .
    
ids:appRoutes 
    a owl:DatatypeProperty;
    rdfs:domain ids:ConfigurationModel;
    rdfs:range xsd:anyURI;
    rdfs:label "App Routes";
    rdfs:comment "Referece to the IRI, where the app routes can be found.";
    .

ids:connectorDescription a owl:DatatypeProperty;
    rdfs:label "connectorDescription"@en;
    rdfs:domain ids:ConfigurationModel;
    rdfs:range ids:Connector; 
    rdfs:comment "The Connector RDF entity referred by the Configuration Model. "@en.
